finish alloc_module_sound

theories/instantiation_properties.v
@@ -4,7 +4,7 @@ From ITree Require Import ITree.
 From ITree Require ITreeFacts.
 From stdpp Require Import list fin_maps gmap base.
 From Wasm Require Import list_extra datatypes datatypes_properties properties
-                         interpreter binary_format_parser operations
+     interpreter binary_format_parser operations type_preservation
                          typing opsem type_checker memory memory_list instantiation.
 Require Export stdpp_aux.
 From Coq Require Import BinNat.
@@ -54,41 +54,6 @@ Print alloc_func.
 
 Print module_func.
 
-(* This is the key definition: we should really be able to tell what the allocated new function closures are from the information of alloc_funcs. However, we need to formulate this in a way that is convenient for the other parts of the proofs. *)
-Definition alloc_funcs_new_closures (modfuncs: list module_func) (inst: instance) : list (function_closure host_function) :=
-  List.map (fun (mf: module_func) => 
-              (FC_func_native inst
-                              (List.nth match mf.(modfunc_type) with
-                                        | Mk_typeidx n => n
-                                        end
-                                        (inst.(inst_types)) (Tf [::] [::]))
-                              mf.(modfunc_locals)
-                              mf.(modfunc_body))) modfuncs.
-
-(* Same for this, but this is easier to define -- we should also be able to tell what the allocated function indices are. *)
-
-(*
-Fixpoint nat_list (acc: list nat) (n : nat) : list nat :=
-  match n with
-  | O => acc
-  | (S n') => nat_list (n' :: acc) n'
-  end.
- 
-Lemma nat_list_length: forall acc n,
-  length (nat_list acc n) = length acc + n.
-Proof.
-Admitted.
-
-Lemma 
-
-i < n -> 
-List.nth_error (nat_list acc n) i = Some i.
-
-Lemma 
-i >= n -> 
-List.nth_error (nat_list acc n) i = List.nth_error acc (i - n).
-*)
-
 Definition gen_index offset len : list nat :=
   imap (fun i x => i+offset+x) (repeat 0 len).
 
@@ -134,65 +99,13 @@ Lemma gen_index_in x offset len:
 Proof.
 Admitted.
 
-(*
-Definition alloc_funcs_new_indices (ws: store_record) (modfuncs: list module_func) : list funcidx :=
-  List.map (fun n => Mk_funcidx (n + List.length ws.(s_funcs))) (nat_list nil (List.length modfuncs)).
- *)
-
-(*
-Definition alloc_funcs_new_indices (ws : store_record) (modfuncs: list module_func) : list funcidx :=
-  List.map Mk_funcidx (gen_index (length (s_funcs ws)) (length modfuncs)).
-
-Lemma alloc_func_ws_res modfuncs ws inst ws' l:
-  (ws', l) = alloc_funcs host_function ws modfuncs inst ->
-  ws'.(s_funcs) = ws.(s_funcs) ++ alloc_funcs_new_closures modfuncs inst /\
-  ws'.(s_tables) = ws.(s_tables) /\
-  ws'.(s_mems) = ws.(s_mems) /\
-  ws'.(s_globals) = ws.(s_globals).
-Proof.
-  move: l ws' ws. Check List.rev_ind.
-  induction modfuncs using List.rev_ind; move => l ws' ws Halloc => /=.
-
-  (* modfuncs = nil *)
-  - inversion Halloc; subst.
-    split => //=; first by rewrite -> List.app_nil_r.
-
-  (* modfuncs = modfuncs ++ [:: x] *)
-  - rewrite /alloc_funcs /alloc_Xs in Halloc.
-    
-    rewrite List.fold_left_app in Halloc.
-    remember (List.fold_left _ modfuncs (ws, [::])) as temp_ws_l.
-    destruct temp_ws_l as [ws_i l_i].
-    
-    simpl in Halloc.
-    specialize (IHmodfuncs (List.rev l_i) ws_i ws). 
-    destruct IHmodfuncs as [Hfunc [Htab [Hmem Hglob]]].
-    {
-      rewrite /alloc_funcs /alloc_Xs.
-      by rewrite <- Heqtemp_ws_l.
-    }
-    {
-      rewrite /add_func in Halloc.
-      inversion Halloc. simpl.
-      split.     
-      + (* s_funcs ws_i ++ x_func_inst = s_funcs ws ++ alloc_funcs_new (modfuncs ++ [:: x]) *)
-        rewrite /alloc_funcs_new_closures.
-        rewrite List.map_app. simpl.
-        rewrite -> List.app_assoc.
-        f_equal. exact Hfunc.
-      + (* s_tables /\ s_mems /\ s_globals *)
-        by split => //=.
-    }
-Qed.
- *)
-
 Definition gen_func_instance mf inst : function_closure host_function :=
   let ft := nth match modfunc_type mf with
                 | Mk_typeidx n => n
                 end (inst_types inst) (Tf [] []) in
   FC_func_native inst ft (modfunc_locals mf) (modfunc_body mf).
 
-Lemma alloc_func_gen_index (modfuncs : list module_func)  ws inst ws' l:
+Lemma alloc_func_gen_index modfuncs ws inst ws' l:
   alloc_funcs host_function ws modfuncs inst = (ws', l) ->
   map (fun x => match x with | Mk_funcidx i => i end) l = gen_index (length (s_funcs ws)) (length modfuncs) /\
   ws'.(s_funcs) = ws.(s_funcs) ++ fmap (fun mf => gen_func_instance mf inst) modfuncs /\
@@ -235,6 +148,217 @@ Proof.
       by rewrite -> list_fmap_app.
 Qed.
 
+Lemma alloc_tab_gen_index modtabtypes ws ws' l:
+  alloc_tabs host_function ws modtabtypes = (ws', l) ->
+  map (fun x => match x with | Mk_tableidx i => i end) l = gen_index (length (s_tables ws)) (length modtabtypes) /\
+  ws'.(s_tables) = ws.(s_tables) ++ fmap (fun '{| tt_limits := {| lim_min := min; lim_max := maxo |} |} => {| table_data := repeat None (ssrnat.nat_of_bin min); table_max_opt := maxo |}) modtabtypes /\
+  ws.(s_funcs) = ws'.(s_funcs) /\
+  ws.(s_mems) = ws'.(s_mems) /\
+  ws.(s_globals) = ws'.(s_globals).
+Proof.
+  unfold alloc_tabs, alloc_Xs.
+  generalize dependent l.
+  generalize dependent ws'.
+  generalize dependent ws.
+  induction modtabtypes using List.rev_ind; move => ws ws' l Halloc.
+  - inversion Halloc; subst; clear Halloc.
+    repeat split => //.
+    simpl.
+    by rewrite app_nil_r.
+  - rewrite fold_left_app in Halloc.
+    remember (fold_left _ modtabtypes (ws,[])) as fold_res.
+    simpl in Halloc.
+    destruct fold_res as [ws0 l0].
+    symmetry in Heqfold_res.
+    unfold alloc_tab, add_table in Halloc.
+    destruct x => /=.
+    destruct tt_limits => /=.
+    specialize (IHmodtabtypes ws ws0 (rev l0)).
+    rewrite Heqfold_res in IHmodtabtypes.
+    inversion Halloc; subst; clear Halloc.
+    simpl in *.
+    rewrite map_app app_length /=.
+    rewrite gen_index_extend.
+    destruct IHmodtabtypes as [? [? [? [? ?]]]] => //.
+    repeat split => //.
+    + rewrite H.
+      rewrite H0.
+      by rewrite app_length map_length.
+    + rewrite H0.
+      rewrite - app_assoc.
+      f_equal.
+      by rewrite -> list_fmap_app => /=.
+Qed.
+
+Lemma alloc_mem_gen_index modmemtypes ws ws' l:
+  alloc_mems host_function ws modmemtypes = (ws', l) ->
+  map (fun x => match x with | Mk_memidx i => i end) l = gen_index (length (s_mems ws)) (length modmemtypes) /\
+  ws'.(s_mems) = ws.(s_mems) ++ fmap (fun '{| lim_min := min; lim_max := maxo |} => {| mem_data := memory_list.mem_make #00%byte (page_size * min)%N; mem_max_opt := maxo |}) modmemtypes /\
+  ws.(s_funcs) = ws'.(s_funcs) /\
+  ws.(s_tables) = ws'.(s_tables) /\
+  ws.(s_globals) = ws'.(s_globals).
+Proof.
+  unfold alloc_mems, alloc_Xs.
+  generalize dependent l.
+  generalize dependent ws'.
+  generalize dependent ws.
+  induction modmemtypes using List.rev_ind; move => ws ws' l Halloc.
+  - inversion Halloc; subst; clear Halloc.
+    repeat split => //=.
+    by rewrite app_nil_r.
+  - rewrite fold_left_app in Halloc.
+    remember (fold_left _ modmemtypes (ws,[])) as fold_res.
+    simpl in Halloc.
+    destruct fold_res as [ws0 l0].
+    symmetry in Heqfold_res.
+    unfold alloc_mem, add_mem in Halloc.
+    destruct x => /=.
+    specialize (IHmodmemtypes ws ws0 (rev l0)).
+    rewrite Heqfold_res in IHmodmemtypes.
+    inversion Halloc; subst; clear Halloc.
+    simpl in *.
+    rewrite map_app app_length /=.
+    rewrite gen_index_extend.
+    destruct IHmodmemtypes as [? [? [? [? ?]]]] => //.
+    repeat split => //.
+    + rewrite H.
+      rewrite H0.
+      by rewrite app_length fmap_length.
+    + rewrite H0.
+      rewrite - app_assoc.
+      f_equal.
+      by rewrite -> list_fmap_app => /=.
+Qed.
+
+Lemma alloc_glob_gen_index modglobs ws g_inits ws' l:
+  length g_inits = length modglobs ->
+  alloc_globs host_function ws modglobs g_inits = (ws', l) ->
+  map (fun x => match x with | Mk_globalidx i => i end) l = gen_index (length (s_globals ws)) (length modglobs) /\
+  ws'.(s_globals) = ws.(s_globals) ++ fmap (fun '({| modglob_type := gt; modglob_init := ge |}, v) => {| g_mut := gt.(tg_mut); g_val := v |} ) (combine modglobs g_inits) /\
+ (* length ws'.(s_globals) = length ws.(s_globals) + length modglobs /\*)
+  ws.(s_funcs) = ws'.(s_funcs) /\
+  ws.(s_tables) = ws'.(s_tables) /\
+  ws.(s_mems) = ws'.(s_mems).
+Proof.
+  (*
+  unfold alloc_globs, alloc_Xs.
+  generalize dependent l.
+  generalize dependent ws'.
+  generalize dependent ws.
+  generalize dependent g_inits.
+  induction modglobs using List.rev_ind; move => g_inits ws ws' l Hlen Halloc.
+  - inversion Halloc; subst; clear Halloc.
+    repeat split => //=.
+    by rewrite app_nil_r.
+  - destruct g_inits using List.rev_ind; first by destruct modglobs => /=.
+    repeat rewrite app_length in Hlen; simpl in Hlen.
+    repeat rewrite - cat_app in Halloc.
+    rewrite combine_app in Halloc; last by lias.
+    simpl in Halloc.
+    rewrite fold_left_app in Halloc.
+    lazymatch goal with
+    | _: context C [fold_left ?f (combine modglobs g_inits) (ws, [])] |- _ =>
+      remember (fold_left f (combine modglobs g_inits) (ws, [])) as fold_res
+    end.
+    (* rewrite - Heqfold_res in Halloc. *)
+    destruct fold_res as [ws0 l0].
+    symmetry in Heqfold_res.
+    unfold alloc_glob, add_glob in Halloc.
+    simpl in Halloc.
+    inversion Halloc; subst; clear Halloc.
+    rewrite map_app app_length /=.
+    rewrite gen_index_extend.
+    specialize (IHmodglobs g_inits ws ws0 (rev l0)).
+    destruct IHmodglobs as [? [? [? [? ?]]]] => //.
+    + by lias.
+    + by rewrite Heqfold_res.
+    repeat split => //.
+    + rewrite H.
+      rewrite H0.
+      rewrite app_length fmap_length combine_length.
+      repeat f_equal.
+      by lias.
+    + rewrite H0.
+      rewrite - app_assoc.
+      f_equal.
+      rewrite combine_app => /=.
+      rewrite -> list_fmap_app => /=.
+      repeat f_equal.
+      destruct x => //.
+      by lias.
+Qed. *) Admitted.
+
+
+Lemma fold_left_preserve {A B: Type} (P: A -> Prop) (f: A -> B -> A) (l: list B) (acc: A) :
+  P acc ->
+  (forall (x:A) (act: B), P x -> P (f x act)) ->
+  P (fold_left f l acc).
+Proof.
+(*
+  (* Check fold_left_rev_right. *)
+  rewrite -fold_left_rev_right.
+  revert acc.
+  induction l;simpl;auto.
+  intros acc Ha Hnext.
+  Locate for
+  rewrite stdpp.list.foldr_snoc /=. apply IHl =>//.
+  apply Hnext=>//.
+Qed.    *)
+ 
+Admitted.
+
+Lemma init_tabs_preserve ws inst e_inits melem ws':
+  init_tabs host_function ws inst e_inits melem = ws' ->
+  ws.(s_funcs) = ws'.(s_funcs) /\
+  ws.(s_mems) = ws'.(s_mems) /\
+  ws.(s_globals) = ws'.(s_globals).
+Proof.
+  move => Hinit.
+  unfold init_tabs in Hinit.
+  rewrite - Hinit.
+  apply fold_left_preserve => //.
+  move => x [n me] Heq.
+  destruct ws, x.
+  simpl in *.
+  destruct Heq as [-> [-> ->]].
+  unfold init_tab => /=.
+  by destruct (nth _ _) eqn:Hl => /=.
+Qed.
+
+Lemma init_tabs_preserve_typing s s' inst m x:
+  store_typing s ->
+  (* instantiate_elem host_function host_instance inst hs' s m x -> *)
+  check_bounds_elem host_function inst s m x ->
+  s' = (init_tabs host_function s inst [seq Z.to_nat (Wasm_int.Int32.intval o) | o <- x] (mod_elem m)) ->
+  store_typing s'.
+Proof.
+Admitted.
+    
+Lemma init_mems_preserve ws inst d_inits mdata ws':
+  init_mems host_function ws inst d_inits mdata = ws' ->
+  ws.(s_funcs) = ws'.(s_funcs) /\
+  ws.(s_tables) = ws'.(s_tables) /\
+  ws.(s_globals) = ws'.(s_globals).
+Proof.
+  move => Hinit.
+  unfold init_mems in Hinit.
+  rewrite - Hinit.
+  apply fold_left_preserve => //.
+  move => x [n md] Heq.
+  destruct ws, x.
+  simpl in *.
+  destruct Heq as [-> [-> ->]].
+  by unfold init_mem => /=.
+Qed.
+
+Lemma init_mems_preserve_typing s inst m x:
+  store_typing s ->
+  (* instantiate_data host_function host_instance inst hs' s m x -> *)
+  check_bounds_data host_function inst s m x ->
+  store_typing (init_mems host_function s inst [seq Z.to_N (Wasm_int.Int32.intval o) | o <- x] (mod_data m)).
+Proof.
+Admitted.
+
 Lemma all2_forward: forall A B (f1 f2 : A -> B -> bool) l1 l2,
   (forall a b, f1 a b -> f2 a b) ->
   (all2 f1 l1 l2 -> all2 f2 l1 l2).
@@ -247,11 +371,6 @@ Proof.
     + by apply E.
     + by apply IH => //=.
 Qed.
-(* 
-all2 g l1 l2 /\ all2 h l1 l2 -> 
-all2 (fun a b => (g a b) && (h a b)) l1 l2 
-
- *)
 
 Lemma all2_and: forall A B (f g h : A -> B -> bool) l1 l2,
     (forall a b, f a b = (g a b) && (h a b)) -> 
@@ -280,12 +399,59 @@ Proof.
     by apply/ssrnat.ltP.
 Qed.
 
+Lemma globals_agree_aux s_globs globs n tg: 
+  globals_agree s_globs n tg ->
+  globals_agree (s_globs ++ globs) n tg.
+Proof.
+  rewrite /globals_agree.
+  move/andP => [H1 H2]. move/eqP in H2.
+  apply/andP. split.
+  + rewrite app_length.
+    by rewrite ssrnat.ltn_addr.
+  + apply/eqP.
+    rewrite <- H2.
+    apply f_equal.
+    apply nth_error_app1.
+    by apply/ssrnat.ltP.
+Qed.
+
+Lemma tabi_agree_aux s_tabs tabs n tt:
+  tabi_agree s_tabs n tt -> 
+  tabi_agree (s_tabs ++ tabs) n tt.
+Proof.
+  rewrite /tabi_agree.
+  move/andP => [H1 H2].
+  apply/andP. split.
+  + rewrite app_length.
+    by rewrite ssrnat.ltn_addr.
+  + assert (H: nth_error (s_tabs ++ tabs) n = nth_error s_tabs n).
+    { apply nth_error_app1. by apply/ssrnat.ltP. }
+    by rewrite -> H.
+Qed.
+
+Lemma memi_agree_aux s_mems mems n tm:
+  memi_agree s_mems n tm -> 
+  memi_agree (s_mems ++ mems) n tm.
+Proof.
+  rewrite /memi_agree.
+  move/andP => [H1 H2].
+  apply/andP. split.
+  + rewrite app_length.
+    by rewrite ssrnat.ltn_addr.
+  + assert (H: nth_error (s_mems ++ mems) n = nth_error s_mems n).
+    { apply nth_error_app1. by apply/ssrnat.ltP. }
+    by rewrite -> H.
+Qed.
+
+
 Let cl_type_check_single := @cl_type_check_single host_function.
 
-Lemma cl_type_check_single_aux s_funcs s_tables s_mems s_globals func funcs:
+Lemma cl_type_check_single_aux s_funcs s_tables s_mems s_globals func funcs tabs mems globs:
   cl_type_check_single {| s_funcs := s_funcs; s_tables := s_tables; s_mems := s_mems; s_globals := s_globals |} func ->
   cl_type_check_single {| s_funcs := s_funcs ++ funcs; 
-                          s_tables := s_tables; s_mems := s_mems; s_globals := s_globals |} func.
+                          s_tables := s_tables ++ tabs;
+                          s_mems := s_mems ++ mems;
+                          s_globals := s_globals ++ globs|} func.
 Proof.
   move => Hcl.
   destruct Hcl as [tf' Hcl_typing].
@@ -314,9 +480,22 @@ Proof.
     apply/andP. split => //=.
     apply/andP. split => //=.
     apply/andP. split => //=.
-    eapply all2_forward.
-    apply functions_agree_aux.
-    by exact Hfunc.
+    - (* functions_agree *)
+      eapply all2_forward.
+      apply functions_agree_aux.
+      by exact Hfunc.
+    - (* globals_agree *)
+      eapply all2_forward.
+      apply globals_agree_aux.
+      by exact Hglb.
+    - (* tabi_agree *)
+      eapply all2_forward.
+      apply tabi_agree_aux.
+      by exact Htab.
+    - (* memi_agree *)
+      eapply all2_forward.
+      apply memi_agree_aux.
+      by exact Hmem.
   + (* cl_typing_host *)
     inversion Hcl_typing; subst.
     by apply cl_typing_host.
@@ -324,10 +503,12 @@ Qed.
 
 Let tab_agree := @tab_agree host_function.
 
-Lemma tab_agree_aux s_funcs s_tables s_mems s_globals tab funcs:
+Lemma tab_agree_aux s_funcs s_tables s_mems s_globals tab funcs tabs mems globs:
   tab_agree {| s_funcs := s_funcs; s_tables := s_tables; s_mems := s_mems; s_globals := s_globals |} tab ->
-  tab_agree {| s_funcs := s_funcs ++ funcs; s_tables := s_tables; s_mems := s_mems;
-               s_globals := s_globals |} tab .
+  tab_agree {| s_funcs := s_funcs ++ funcs;
+               s_tables := s_tables ++ tabs;
+               s_mems := s_mems ++ mems;
+               s_globals := s_globals ++ globs |} tab .
 Proof.
   rewrite /tab_agree /typing.tab_agree.
   move => Htb.
@@ -348,15 +529,6 @@ Proof.
     assumption.
 Qed.
 
-(*
-Lemma forall2_length: forall A B R (l1 : seq.seq A) (l2 : seq.seq B),
-    List.Forall2 R l1 l2 -> List.length l1 = List.length l2.
-Proof.
-Admitted.
- *)
-
-
-
 Lemma nth_error_lookup {T: Type} (l: list T) i:
   nth_error l i = l !! i.
 Proof.
@@ -376,7 +548,11 @@ Lemma Forall2_nth_error: forall A B R (l1 : seq.seq A) (l2 : seq.seq B) n m k,
     List.nth_error l2 n = Some k ->
     R m k.
 Proof.
-Admitted.
+  move => A B R l1 l2 n m k HForall2 Hnth1 Hnth2.
+  rewrite nth_error_lookup in Hnth1.
+  rewrite nth_error_lookup in Hnth2.
+  by eapply Forall2_lookup_lr.
+Qed.
 
 
 Search Forall2.
@@ -394,49 +570,755 @@ Lemma Forall2_lift: forall A B (R : A -> B -> Prop) (l1 : seq.seq A) (l2 : seq.s
     R m k) ->
     List.Forall2 R l1 l2.
 Proof.
-Admitted.
-
+  move => A B R l1 l2 Hlen HR.
+  apply Forall2_same_length_lookup_2 => //.
+  move => i x y Hl1 Hl2.
+  rewrite <- nth_error_lookup in Hl1.
+  rewrite <- nth_error_lookup in Hl2.
+  by eapply HR.
+Qed.
 
 Lemma Forall2_all2: forall A B (R : A -> B -> bool ) (l1 : seq.seq A) (l2 : seq.seq B),
     List.Forall2 R l1 l2 = all2 R l1 l2.
 Proof.
+  move => A B R l1.
+  induction l1.
+  - destruct l2.
 Admitted.
 
 
-Lemma alloc_func_sound s s' ifs mod_funcs mod_types fts inst t_context: 
-  (s', ifs) = alloc_funcs host_function s mod_funcs inst ->
-  List.Forall2 (module_func_typing t_context) mod_funcs fts ->
-  t_context.(tc_func_t) = fts ->
-  t_context.(tc_types_t) = mod_types ->
-  t_context.(tc_global) = nil ->
-  t_context.(tc_table) = nil -> 
-  t_context.(tc_memory) = nil ->
-  t_context.(tc_local) = nil ->
-  t_context.(tc_label) = nil ->
-  t_context.(tc_return) = None ->
-  inst.(inst_types) = mod_types ->
-  inst.(inst_funcs) = List.map (fun '(Mk_funcidx i) => i) ifs ->
-  inst.(inst_globs) = nil ->
-  inst.(inst_tab) = nil ->
-  inst.(inst_memory) = nil -> 
-  store_typing s ->
+Lemma nth_error_same_length_list:
+  forall (A B : Type) (l1 : seq.seq A) (l2 : seq.seq B) (i : nat) (m : A),
+     length l1 = length l2 ->
+     nth_error l1 i = Some m -> 
+     exists n, nth_error l2 i = Some n.
+Proof.
+  move => A B l1 l2 i m.
+Admitted.
+
+
+Check nth_error_Some.
+
+Lemma nth_error_Some_length:
+  forall A (l : seq.seq A) (i : nat) (m : A),
+  nth_error l i = Some m -> 
+  i < length l.
+Proof.
+  move => A l i m H1.
+  assert (H2 : nth_error l i ≠ None) by rewrite H1 => //.
+  by apply List.nth_error_Some in H2.
+Qed.
+
+
+Lemma external_typing_aux s v_imps t_imps:
+  Forall2 (instantiation.external_typing host_function s) v_imps t_imps -> 
+  length (ext_funcs v_imps) = length (ext_t_funcs t_imps) /\
+  length (ext_globs v_imps) = length (ext_t_globs t_imps) /\
+  length (ext_tabs v_imps) = length (ext_t_tabs t_imps) /\
+  length (ext_mems v_imps) = length (ext_t_mems t_imps).
+Proof.
+  generalize t_imps.
+  induction v_imps as [| v_imp v_imps' IH ].
+  - move => t_imps' H.
+    apply Forall2_length in H.
+    simpl in H. symmetry in H.
+    apply nil_length_inv in H.
+    by rewrite H.
+  - clear t_imps. move => t_imps H.
+    inversion H; subst.
+    rewrite /ext_funcs /ext_t_funcs.
+    repeat split; inversion H2; subst; simpl; f_equal; by apply IH.
+Qed.
+
+(*
+Lemma external_typing_proj s n v_imps v_imp t_imps t_imp:
+  Forall2 (instantiation.external_typing host_function s) v_imps t_imps ->
+  Forall2 (instantiation.external_typing host_function s) (map (λ '(MED_func (Mk_funcidx i)), i) (ext_funcs v_imps)) (map (λ '(ET_func tf), tf) (ext_t_funcs t_imps)).
+Proof.
+Admitted.
+ *)
+
+      
+
+Lemma tab_agree_from_typing mod_tables s_tabs s :
+  all module_tab_typing mod_tables -> 
+  s_tabs = (λ '{| tt_limits := {| lim_min := min; lim_max := maxo |} |},
+               {| table_data := repeat None (ssrnat.nat_of_bin min); table_max_opt := maxo |})
+                 <$> map (λ t : module_table, modtab_type t) mod_tables ->
+  Forall (typing.tab_agree (host_function:=host_function) s) s_tabs.
+Proof.
+  move => HTabType Heqs_tabs_new.
+  rewrite List.Forall_forall => ti Hin.
+      
+  rewrite -> Heqs_tabs_new in Hin.
+  eapply List.In_nth_error in Hin.
+  destruct Hin as [n Hnth].
+  rewrite Coqlib.list_map_nth in Hnth.
+  rewrite /Coqlib.option_map in Hnth.
+  destruct (nth_error (map (λ t : module_table, modtab_type t) mod_tables) n) eqn: Heqt => //=.
+  inversion Hnth. clear Hnth.
+  rename H0 into Heq_ti.
+
+  assert (Hex_tab: exists tab, nth_error mod_tables n = Some tab).
+  {
+    eapply nth_error_same_length_list with (l1 := (map (λ t : module_table, modtab_type t) mod_tables)) => //.
+    by rewrite map_length.
+  }
+  destruct Hex_tab as [tab Htab].
+
+  rewrite /module_tab_typing in HTabType.
+  eapply list_all_forall in HTabType; last by apply Coqlib.nth_error_in in Htab.
+
+  apply map_nth_error with (f := (λ t : module_table, modtab_type t)) in Htab.
+  rewrite Heqt in Htab.
+  inversion Htab. 
+  rewrite <- H0 in HTabType. rewrite <- H0.
+  clear Htab H0.
+
+  rewrite /limit_typing in HTabType.
+
+  destruct t. simpl in HTabType.
+  destruct tt_limits.
+
+  move/andP in HTabType. destruct HTabType as [Hmax Hmin].
+
+  rewrite /typing.tab_agree. simpl.
+  split.
+  * (* tabcl_agree *)
+    apply Forall_forall => lim Hin.
+    apply repeat_spec in Hin.
+    rewrite /tabcl_agree.
+    by rewrite Hin.
+  * (* tabsize_agree *)
+    rewrite /tabsize_agree. simpl.
+    destruct lim_max as [max | ] => //.
+    rewrite /tab_size. simpl.
+    rewrite repeat_length.
+    destruct lim_min as [ | min].
+    -- simpl.
+       by apply ssrnat.leq0n.
+    -- apply/ssrnat.leP.
+       move/N.leb_spec0 in Hmin.
+Admitted.
+
+
+Lemma mem_agree_from_typing mod_mems s_mems:
+  all module_mem_typing mod_mems ->
+  s_mems = (λ '{| lim_min := min; lim_max := maxo |},
+               {| mem_data := mem_make #00 match min with
+                                      | 0%N => 0%N
+                                      | N.pos q => N.pos (64 * 1024 * q)
+                                      end;
+                  mem_max_opt := maxo |}) <$> mod_mems ->
+  Forall mem_agree s_mems.
+Proof.
+  move => HMemType Heqs_mems.
+
+  rewrite List.Forall_forall => mi Hin.
+
+  rewrite -> Heqs_mems in Hin.
+  eapply List.In_nth_error in Hin.
+  destruct Hin as [n Hnth].
+  rewrite Coqlib.list_map_nth in Hnth.
+  rewrite /Coqlib.option_map in Hnth.
+  simpl in Hnth.
+  destruct (nth_error mod_mems n) eqn: Heqm; last by rewrite Heqm in Hnth; inversion Hnth.
+    
+  rewrite /module_mem_typing in HMemType.
+  eapply list_all_forall in HMemType; last by apply Coqlib.nth_error_in in Heqm.
+  rewrite Heqm in Hnth.
+  inversion Hnth; subst. clear Hnth.
+
+  rewrite /limit_typing in HMemType.
+  destruct m. simpl in HMemType.
+
+  rewrite /mem_agree. simpl.
+  destruct lim_max as [max | ] => //.
+  rewrite /mem_size /operations.mem_length /memory_list.mem_length.
+  simpl.
+  rewrite repeat_length.
+  rewrite N2Nat.id.
+  rewrite /page_size.
+  destruct lim_min as [ | min].
+  + rewrite N.div_0_l => //.
+    by apply N.le_0_l.
+  + replace (N.pos (64 * 1024 * min)) with (N.mul (N.pos (64 * 1024)) (N.pos min)); last by simpl.
+    rewrite N.mul_comm.
+    replace (N.div (N.pos min * N.pos (64 * 1024)) (64 * 1024)) with (N.pos min); last by symmetry; apply N.div_mul.
+    move/andP in HMemType. destruct HMemType as [_ HMemType].
+    by apply/N.leb_spec0.
+Qed.
+
+Lemma ext_funcs_lookup_exist (modexps: list module_export_desc) n fn:
+  (ext_funcs modexps) !! n = Some fn ->
+  exists k, modexps !! k = Some (MED_func fn).
+Proof.
+  move: n fn.
+  induction modexps; move => n tn Hextfunclookup => //=.
+  simpl in Hextfunclookup.
+  destruct a => //. 
+  { simpl in *.
+       destruct n; simpl in *; first by inversion Hextfunclookup; subst; exists 0.
+       apply IHmodexps in Hextfunclookup.
+       destruct Hextfunclookup as [k ?].
+       by exists (S k).
+  }
+  all: simpl in *. 
+  all: apply IHmodexps in Hextfunclookup.
+  all: destruct Hextfunclookup as [k ?].
+  all: by exists (S k).
+Qed.
+
+Lemma ext_tabs_lookup_exist (modexps: list module_export_desc) n tn:
+  (ext_tabs modexps) !! n = Some tn ->
+  exists k, modexps !! k = Some (MED_table tn).
+Proof.
+  move: n tn.
+  induction modexps; move => n tn Hexttablookup => //=.
+  simpl in Hexttablookup.
+  destruct a => //. 
+  2: { simpl in *.
+       destruct n; simpl in *; first by inversion Hexttablookup; subst; exists 0.
+       apply IHmodexps in Hexttablookup.
+       destruct Hexttablookup as [k ?].
+       by exists (S k).
+  }
+  all: simpl in *. 
+  all: apply IHmodexps in Hexttablookup.
+  all: destruct Hexttablookup as [k ?].
+  all: by exists (S k).
+Qed.
+
+Lemma ext_mems_lookup_exist (modexps: list module_export_desc) n mn:
+  (ext_mems modexps) !! n = Some mn ->
+  exists k, modexps !! k = Some (MED_mem mn).
+Proof.
+  move: n mn.
+  induction modexps; move => n mn Hextmemlookup => //=.
+  simpl in Hextmemlookup.
+  destruct a => //. 
+  3: { simpl in *.
+       destruct n; simpl in *; first try by inversion Hextmemlookup; subst; exists 0.
+       apply IHmodexps in Hextmemlookup.
+       destruct Hextmemlookup as [k ?].
+       by exists (S k).
+  }
+  all: simpl in *. 
+  all: apply IHmodexps in Hextmemlookup.
+  all: destruct Hextmemlookup as [k ?].
+  all: by exists (S k).
+Qed.
+
+Lemma ext_globs_lookup_exist (modexps: list module_export_desc) n fn:
+  (ext_globs modexps) !! n = Some fn ->
+  exists k, modexps !! k = Some (MED_global fn).
+Proof.
+  move: n fn.
+  induction modexps; move => n tn Hextgloblookup => //=.
+  simpl in Hextgloblookup.
+  destruct a => //. 
+  4: { simpl in *.
+       destruct n; simpl in *; first by inversion Hextgloblookup; subst; exists 0.
+       apply IHmodexps in Hextgloblookup.
+       destruct Hextgloblookup as [k ?].
+       by exists (S k).
+  }
+  all: simpl in *. 
+  all: apply IHmodexps in Hextgloblookup.
+  all: destruct Hextgloblookup as [k ?].
+  all: by exists (S k).
+Qed.
+
+Lemma bet_const_exprs_len tc es t1 t2:
+  const_exprs tc es ->
+  be_typing tc es (Tf t1 t2) ->
+  length t2 = length es + length t1.
+Proof.
+  (*
+  move: t1 t2.
+  induction es; move => t1 t2 Hconst Hbet; destruct t2 => //=.
+  { apply empty_typing in Hbet. by subst. }
+  { apply empty_typing in Hbet. by subst. }
+  { rewrite <- cat1s in Hbet.
+    apply composition_typing in Hbet.
+    destruct Hbet as [ts [t1s [t2s [t3s [-> [Heqt2 [Hbet1 Hbet2]]]]]]].
+    destruct ts, t2s => //=.
+    simpl in Hconst.
+    move/andP in Hconst.
+    destruct Hconst as [Hconst Hconsts].
+    apply IHes in Hbet2 => //.
+    destruct es, t3s => //=.
+    unfold const_expr in Hconst.
+    destruct a => //.
+    { apply Get_global_typing in Hbet1.
+      destruct Hbet1 as [t [? [HContra ?]]].
+      by destruct t1s.
+    }
+    { apply BI_const_typing in Hbet1.
+      by destruct t1s.
+    }
+  }
+  { rewrite <- cat1s in Hbet.
+    apply composition_typing in Hbet.
+    destruct Hbet as [ts [t1s [t2s [t3s [-> [Heqt2 [Hbet1 Hbet2]]]]]]].
+    simpl in Hconst.
+    move/andP in Hconst.
+    destruct Hconst as [Hconst Hconsts].
+    eapply IHes in Hconsts => //.
+    f_equal.
+    assert (length t2 + 1 = length ts + length t2s) as Hlent2.
+    { rewrite <- app_length.
+      rewrite <- cat_app.
+      rewrite <- Heqt2.
+      by lias.
+    }
+    unfold const_expr in Hconst.
+    destruct a => //.
+    { apply Get_global_typing in Hbet1.
+      destruct Hbet1 as [t [? [HContra ?]]].
+      subst.
+      rewrite -> app_length in *.
+      simpl in *.
+      by lias.
+    }
+    { apply BI_const_typing in Hbet1.
+      subst.
+      rewrite -> app_length in *.
+      simpl in *.
+      by lias.
+    }
+  }
+Qed.*) Admitted.
+  
+Lemma const_exprs_impl tc es t:
+  const_exprs tc es ->
+  be_typing tc es (Tf [] [::t]) ->
+  exists e, es = [:: e] /\ const_expr tc e.
+Proof.
+  move => Hconst Hbet.
+  eapply bet_const_exprs_len in Hbet => //.
+  do 2 destruct es => //=.
+  exists b; split => //.
+  unfold const_exprs in Hconst.
+  simpl in Hconst.
+  move/andP in Hconst.
+  by destruct Hconst.
+Qed.
+
+Check reduce_trans.
+Lemma reduce_trans_const hs s1 f1 v1 s2 f2 v2:
+  reduce_trans (host_instance:=host_instance) (hs, s1, f1, [AI_basic (BI_const v1)]) (hs, s2, f2, [AI_basic (BI_const v2)]) ->
+  v1 = v2.
+Proof.
+  (*
+  move => Hred.
+  unfold reduce_trans in Hred.
+  apply Operators_Properties.clos_rt_rt1n_iff in Hred.
+  inversion Hred => //.
+  unfold reduce_tuple in H.
+  destruct y as [[??]?].
+  by apply const_no_reduce in H.
+Qed.
+   *) Admitted.
+Check sglob_val. Locate sglob_val.
+
+Lemma reduce_trans_get_global hs s f s' f' i v:
+  reduce_trans (host_instance:=host_instance) (hs, s, f, [AI_basic (BI_get_global i)]) (hs, s', f', [AI_basic (BI_const v)]) ->
+  sglob_val s (f_inst f) i = Some v.
+Proof.
+  (*
+  move => Hred.
+  unfold reduce_trans in *.
+  apply Operators_Properties.clos_rt_rt1n_iff in Hred.
+  inversion Hred; subst; clear Hred.
+  destruct y as [[??]?].
+  unfold reduce_tuple in H.
+  apply reduce_get_global in H.
+  destruct H as [v' [Hsgv ->]].
+  inversion H0; subst; clear H0 => //.
+  unfold reduce_tuple in H.
+  destruct y as [[??]?].
+  by apply const_no_reduce in H.
+Qed. *) Admitted.
+
+Lemma external_typing_func s v_imps t_imps n v_imp t_imp:
+  nth_error (map (λ '(Mk_funcidx i), i) (ext_funcs v_imps)) n = Some v_imp ->
+  nth_error (ext_t_funcs t_imps) n = Some t_imp -> 
+  instantiation.external_typing host_function s (MED_func (Mk_funcidx v_imp)) (ET_func t_imp) ->
+  option_map cl_type (nth_error (s_funcs s) v_imp) = Some t_imp.
+Proof.
+  move => Hvimp Htimp Htyping.
+  inversion Htyping; subst.
+  by rewrite H3.
+Qed.
+
+
+Lemma external_typing_tab s v_imps t_imps n v_imp t_imp:
+  nth_error (map (λ '(Mk_tableidx i), i) (ext_tabs v_imps)) n = Some v_imp ->
+  nth_error (ext_t_tabs t_imps) n = Some t_imp -> 
+  instantiation.external_typing host_function s (MED_table (Mk_tableidx v_imp)) (ET_tab t_imp) ->
+  exists ti, (nth_error (s_tables s) v_imp = Some ti) /\
+          tab_typing ti t_imp.
+Proof.
+  move => Hvimp Htimp Htyping.
+  inversion Htyping; subst.
+  exists ti. split => //=.
+Qed.
+
+
+Definition module_export_entity_relate (R : module_export_desc → extern_t → Prop) : Prop :=
+  forall vi ti, R vi ti ->
+           match vi with
+           | MED_func _ => match ti with
+                          | ET_func _ => True
+                          | _ => False
+                          end
+           | MED_table _ => match ti with
+                           | ET_tab _ => True
+                           | _ => False
+                           end                             
+           | MED_mem _ => match ti with
+                         | ET_mem _ => True
+                         | _ => False
+                         end
+           | MED_global _ => match ti with
+                            | ET_glob _ => True
+                            | _ => False
+                            end                            
+           end.
+
+Lemma external_typing_relate s :
+  module_export_entity_relate (instantiation.external_typing host_function s).
+Proof.
+  rewrite /module_export_entity_relate => vi ti HR.
+  inversion HR => //.
+Qed.
+  
+Lemma vt_imps_funcs_lookup R v_imps t_imps fn ft (k: nat):
+  module_export_entity_relate R ->
+  Forall2 R v_imps t_imps ->
+  (ext_funcs v_imps) !! k = Some fn ->
+  (ext_t_funcs t_imps) !! k = Some ft ->
+  exists n, v_imps !! n = Some (MED_func fn) /\ t_imps !! n = Some (ET_func ft).
+Proof.
+  move: t_imps k.
+  induction v_imps; move => t_imps k HR HForall2 Hext_vl Hext_tl => //=.
+  inversion HForall2; subst.
+  specialize (HR a y H1) as H2.
+  destruct a; destruct y; simpl in * => //.
+  { destruct k => //.
+    + exists 0. simpl in *.      
+      inversion Hext_vl; subst.
+      by inversion Hext_tl.
+    + simpl in *.
+      specialize (IHv_imps l' k HR H3 Hext_vl Hext_tl).
+      destruct IHv_imps as [n Hvimp Htimp].
+      by exists (S n).
+  }
+  all: specialize (IHv_imps l' k HR H3 Hext_vl Hext_tl).
+  all: destruct IHv_imps as [n Hvimp Htimp].
+  all: by exists (S n).
+Qed.
+
+Lemma vt_imps_funcs_relate v_imps t_imps fn ft (k: nat) R:
+  module_export_entity_relate R ->
+  Forall2 R v_imps t_imps ->
+  (ext_funcs v_imps) !! k = Some fn ->
+  (ext_t_funcs t_imps) !! k = Some ft ->
+  R (MED_func fn) (ET_func ft).
+Proof.
+  move => HR HForall2 Hvl Htl.
+  eapply vt_imps_funcs_lookup in Hvl => //.
+  destruct Hvl as [n [Hvl' Htl']].
+  rewrite -> Forall2_lookup in HForall2.
+  specialize (HForall2 n).
+  rewrite Hvl' Htl' in HForall2 => //.
+  by inversion HForall2.
+Qed.
+
+Lemma external_typing_funcs_aux s n v_imps v_imp t_imps t_imp:
+  Forall2 (instantiation.external_typing host_function s) v_imps t_imps ->
+  nth_error (map (λ '(Mk_funcidx i), i) (ext_funcs v_imps)) n = Some v_imp ->
+  nth_error (ext_t_funcs t_imps) n = Some t_imp -> 
+  option_map cl_type (nth_error (s_funcs s) v_imp) = Some t_imp. 
+Proof.
+  move => Htyping Hmvimps_nth Htimps_nth.
+  rewrite Coqlib.list_map_nth in Hmvimps_nth.
+  rewrite /Coqlib.option_map in Hmvimps_nth.
+  destruct (nth_error (ext_funcs v_imps) n) eqn: Hvimps_nth => //.
+  destruct f as [fidx]. inversion Hmvimps_nth.
+  rewrite <- H0 in *. clear Hmvimps_nth H0.
+  rewrite nth_error_lookup in Htimps_nth.
+  rewrite nth_error_lookup in Hvimps_nth.
+  specialize (external_typing_relate s) as HR.
+  specialize (vt_imps_funcs_relate _ _ _ _ _ _ HR Htyping Hvimps_nth Htimps_nth) as Htyping_n.
+  inversion Htyping_n; subst.
+  rewrite /option_map.
+  by rewrite H3.
+Qed.
+
+Lemma vt_imps_globs_lookup v_imps t_imps gn gt (k: nat) R:
+  module_export_entity_relate R ->
+  Forall2 R v_imps t_imps ->
+  (ext_globs v_imps) !! k = Some gn ->
+  (ext_t_globs t_imps) !! k = Some gt ->
+  exists n, v_imps !! n = Some (MED_global gn) /\ t_imps !! n = Some (ET_glob gt).
+Proof.
+  move: t_imps k.
+  induction v_imps; move => t_imps k HR HForall2 Hext_vl Hext_tl => //=.
+  inversion HForall2; subst.
+  specialize (HR a y H1) as H2.
+  destruct a; destruct y; simpl in * => //.
+  4 : { destruct k => //.
+        + exists 0. simpl in *.      
+          inversion Hext_vl; subst.
+          by inversion Hext_tl; subst.
+        + simpl in *.
+          specialize (IHv_imps l' k HR H3 Hext_vl Hext_tl).
+          destruct IHv_imps as [n Hvimp Htimp].
+          by exists (S n).
+  }
+  all: specialize (IHv_imps l' k HR H3 Hext_vl Hext_tl).
+  all: destruct IHv_imps as [n Hvimp Htimp].
+  all: by exists (S n).
+Qed.
+
+Lemma vt_imps_globs_relate v_imps t_imps gn gt (k: nat) R:
+  module_export_entity_relate R ->
+  Forall2 R v_imps t_imps ->
+  (ext_globs v_imps) !! k = Some gn ->
+  (ext_t_globs t_imps) !! k = Some gt ->
+  R (MED_global gn) (ET_glob gt).
+Proof.
+  move => HR HForall2 Hvl Htl.
+  eapply vt_imps_globs_lookup in Hvl => //.
+  destruct Hvl as [n [Hvl' Htl']].
+  rewrite -> Forall2_lookup in HForall2.
+  specialize (HForall2 n).
+  rewrite Hvl' Htl' in HForall2 => //.
+  by inversion HForall2.
+Qed.
+
+Lemma external_typing_globs_aux s n v_imps v_imp t_imps t_imp:
+  Forall2 (instantiation.external_typing host_function s) v_imps t_imps ->
+  nth_error (map (λ '(Mk_globalidx i), i) (ext_globs v_imps)) n = Some v_imp ->
+  nth_error (ext_t_globs t_imps) n = Some t_imp ->
+  option_map (λ g : global, global_agree g t_imp) (nth_error (s_globals s) v_imp) = Some true. 
+Proof.
+  move => Htyping Hmvimps_nth Htimps_nth.
+  rewrite Coqlib.list_map_nth in Hmvimps_nth.
+  rewrite /Coqlib.option_map in Hmvimps_nth.
+  destruct (nth_error (ext_globs v_imps) n) eqn: Hvimps_nth => //.
+  destruct g as [gidx]. inversion Hmvimps_nth.
+  rewrite <- H0 in *. clear Hmvimps_nth H0.
+  rewrite nth_error_lookup in Htimps_nth.
+  rewrite nth_error_lookup in Hvimps_nth.
+  specialize (external_typing_relate s) as HR.
+  specialize (vt_imps_globs_relate _ _ _ _ _ _ HR Htyping Hvimps_nth Htimps_nth) as Htyping_n.
+  inversion Htyping_n; subst.
+  rewrite /option_map.
+  rewrite H3. by rewrite H4.
+Qed.
+
+Lemma vt_imps_tabs_lookup v_imps t_imps tn tt (k: nat) R:
+  module_export_entity_relate R ->
+  Forall2 R v_imps t_imps ->
+  (ext_tabs v_imps) !! k = Some tn ->
+  (ext_t_tabs t_imps) !! k = Some tt ->
+  exists n, v_imps !! n = Some (MED_table tn) /\ t_imps !! n = Some (ET_tab tt).
+Proof.
+  move: t_imps k.
+  induction v_imps; move => t_imps k HR HForall2 Hext_vl Hext_tl => //=.
+  inversion HForall2; subst.
+  specialize (HR a y H1) as H2.
+  destruct a; destruct y; simpl in * => //.
+  2 : { destruct k => //.
+        + exists 0. simpl in *.      
+          inversion Hext_vl; subst.
+          by inversion Hext_tl; subst.
+        + simpl in *.
+          specialize (IHv_imps l' k HR H3 Hext_vl Hext_tl).
+          destruct IHv_imps as [n Hvimp Htimp].
+          by exists (S n).
+  }
+  all: specialize (IHv_imps l' k HR H3 Hext_vl Hext_tl).
+  all: destruct IHv_imps as [n Hvimp Htimp].
+  all: by exists (S n).
+Qed.
+
+Lemma vt_imps_tabs_relate v_imps t_imps tn tt (k: nat) R:
+  module_export_entity_relate R ->
+  Forall2 R v_imps t_imps ->
+  (ext_tabs v_imps) !! k = Some tn ->
+  (ext_t_tabs t_imps) !! k = Some tt ->
+  R (MED_table tn) (ET_tab tt).
+Proof.
+  move => HR HForall2 Hvl Htl.
+  eapply vt_imps_tabs_lookup in Hvl => //.
+  destruct Hvl as [n [Hvl' Htl']].
+  rewrite -> Forall2_lookup in HForall2.
+  specialize (HForall2 n).
+  rewrite Hvl' Htl' in HForall2 => //.
+  by inversion HForall2.
+Qed.
+
+Lemma external_typing_tabs_aux s n v_imps v_imp t_imps t_imp:
+  Forall2 (instantiation.external_typing host_function s) v_imps t_imps ->
+  nth_error (map (λ '(Mk_tableidx i), i) (ext_tabs v_imps)) n = Some v_imp ->
+  nth_error (ext_t_tabs t_imps) n = Some t_imp ->
+  tabi_agree (s_tables s) v_imp t_imp.
+Proof.
+  move => Htyping Hmvimps_nth Htimps_nth.
+  rewrite Coqlib.list_map_nth in Hmvimps_nth.
+  rewrite /Coqlib.option_map in Hmvimps_nth.
+  destruct (nth_error (ext_tabs v_imps) n) eqn: Hvimps_nth => //.
+  destruct t as [tidx]. inversion Hmvimps_nth.
+  rewrite <- H0 in *. clear Hmvimps_nth H0.
+  rewrite nth_error_lookup in Htimps_nth.
+  rewrite nth_error_lookup in Hvimps_nth.
+  specialize (external_typing_relate s) as HR.
+  specialize (vt_imps_tabs_relate _ _ _ _ _ _ HR Htyping Hvimps_nth Htimps_nth) as Htyping_n.
+  inversion Htyping_n; subst.
+  rewrite /option_map.
+  rewrite /tabi_agree.
+  apply/andP. split => //.
+  by rewrite H3.
+Qed.
+
+Lemma vt_imps_mems_lookup v_imps t_imps tn tt (k: nat) R:
+  module_export_entity_relate R ->
+  Forall2 R v_imps t_imps ->
+  (ext_mems v_imps) !! k = Some tn ->
+  (ext_t_mems t_imps) !! k = Some tt ->
+  exists n, v_imps !! n = Some (MED_mem tn) /\ t_imps !! n = Some (ET_mem tt).
+Proof.
+  move: t_imps k.
+  induction v_imps; move => t_imps k HR HForall2 Hext_vl Hext_tl => //=.
+  inversion HForall2; subst.
+  specialize (HR a y H1) as H2.
+  destruct a; destruct y; simpl in * => //.
+  3 : { destruct k => //.
+        + exists 0. simpl in *.      
+          inversion Hext_vl; subst.
+          by inversion Hext_tl; subst.
+        + simpl in *.
+          specialize (IHv_imps l' k HR H3 Hext_vl Hext_tl).
+          destruct IHv_imps as [n Hvimp Htimp].
+          by exists (S n).
+  }
+  all: specialize (IHv_imps l' k HR H3 Hext_vl Hext_tl).
+  all: destruct IHv_imps as [n Hvimp Htimp].
+  all: by exists (S n).
+Qed.
+
+Lemma vt_imps_mems_relate v_imps t_imps mn mt (k: nat) R:
+  module_export_entity_relate R ->
+  Forall2 R v_imps t_imps ->
+  (ext_mems v_imps) !! k = Some mn ->
+  (ext_t_mems t_imps) !! k = Some mt ->
+  R (MED_mem mn) (ET_mem mt).
+Proof.
+  move => HR HForall2 Hvl Htl.
+  eapply vt_imps_mems_lookup in Hvl => //.
+  destruct Hvl as [n [Hvl' Htl']].
+  rewrite -> Forall2_lookup in HForall2.
+  specialize (HForall2 n).
+  rewrite Hvl' Htl' in HForall2 => //.
+  by inversion HForall2.
+Qed.
+
+Lemma external_typing_mems_aux s n v_imps v_imp t_imps t_imp:
+  Forall2 (instantiation.external_typing host_function s) v_imps t_imps ->
+  nth_error (map (λ '(Mk_memidx i), i) (ext_mems v_imps)) n = Some v_imp ->
+  nth_error (ext_t_mems t_imps) n = Some t_imp ->
+  memi_agree (s_mems s) v_imp t_imp.
+Proof.
+  move => Htyping Hmvimps_nth Htimps_nth.
+  rewrite Coqlib.list_map_nth in Hmvimps_nth.
+  rewrite /Coqlib.option_map in Hmvimps_nth.
+  destruct (nth_error (ext_mems v_imps) n) eqn: Hvimps_nth => //.
+  destruct m as [midx]. inversion Hmvimps_nth.
+  rewrite <- H0 in *. clear Hmvimps_nth H0.
+  rewrite nth_error_lookup in Htimps_nth.
+  rewrite nth_error_lookup in Hvimps_nth.
+  specialize (external_typing_relate s) as HR.
+  specialize (vt_imps_mems_relate _ _ _ _ _ _ HR Htyping Hvimps_nth Htimps_nth) as Htyping_n.
+  inversion Htyping_n; subst.
+  rewrite /memi_agree.
+  apply/andP. split => //.
+  by rewrite H3.
+Qed. 
+
+Lemma alloc_module_sound s s' m v_imps t_imps v_exps t_exps inst gvs hs: 
+  alloc_module host_function s m v_imps gvs (s', inst, v_exps) ->
+  module_typing m t_imps t_exps ->
+  Forall2 (instantiation.external_typing host_function s) v_imps t_imps -> 
+  instantiate_globals host_function host_instance inst hs s' m gvs -> 
+  store_typing s -> 
   store_typing s'.
 Proof.
-  destruct inst, t_context.
-  move => Halloc Hftstype ? ? ? ? ? ? ? ? ? ? ? ? ? Hstoretype; simpl in *; subst.
-  
-  (* Doing induction on mod_funcs is hard since we only have the module validity result for the original module. 
-     Instead, note that we can explicitly evaluate what the new store s' is -- intuitively, it should only differ with the original store in the function component, where a few functions are appended. *)
-  
-  specialize (alloc_func_gen_index _ _ _ _ _ (symmetry Halloc)) as Hfuncidx.
-  destruct Hfuncidx as [Hidx [Hfunc [Htab [Hmem Hglob]]]].
+  move => Halloc Hmod_typing Himp_typing Hinit_globs Hstore_typing.
+  rewrite /module_typing in Hmod_typing.
+  destruct m.
+  destruct Hmod_typing as [fts [gts [HFuncType [HTabType [HMemType [HGlobType [HElemType [HDataType [HStartValid [HImpValid HExpValid]]]]]]]]]].
 
-  (* We have established a relationship between the new store and the old store without using fold_left. We now have to prove the rest. Some of the lemmas proven previously commented out for now) is applicable, but need to be in a more generalised form. *)
+  rewrite /alloc_module in Halloc. simpl in *.
+  remember (alloc_funcs host_function s mod_funcs inst) as s_ifs.
+  destruct s_ifs as [s1 ifs].
+  remember (alloc_tabs host_function s1 (map (λ t : module_table, modtab_type t) mod_tables)) as s_its.
+  destruct s_its as [s2 its].
+  remember (alloc_mems host_function s2 mod_mems) as s_ims.
+  destruct s_ims as [s3 ims].
+  remember (alloc_globs host_function s3 mod_globals gvs) as s_igs.
+  destruct s_igs as [s_end igs].
+
+  destruct inst. simpl in *.
   
-  destruct s'. destruct s. simpl in *. destruct Hstoretype as [Hcl [Htab_agree Hmem_agree]].
-  split; rewrite -> Hfunc; subst.
+  repeat (move/andP in Halloc; destruct Halloc as [Halloc ?]).
+  move/eqP in H; subst.
+  move/eqP in H0; subst.
+  move/eqP in H1; subst.
+  move/eqP in H2; subst.
+  move/eqP in H3; subst.
+  move/eqP in H4; subst.
+  move/eqP in Halloc; subst.
+  
+  destruct s_end. destruct s. simpl in *. destruct Hstore_typing as [Hcl [Htab_agree Hmem_agree]].
+  specialize (alloc_func_gen_index _ _ _ _ _ (symmetry Heqs_ifs)) as Hfuncidx.
+  destruct Hfuncidx as [Hfunidx [Hfunc1 [Htab1 [Hmem1 Hglob1]]]]; simpl in *.
+  specialize (alloc_tab_gen_index _ _ _ _ (symmetry Heqs_its)) as Htabidx.
+  destruct Htabidx as [Htabidx [Htab2 [Hfunc2 [Hmem2 Hglob2]]]]; simpl in *.
+  specialize (alloc_mem_gen_index _ _ _ _ (symmetry Heqs_ims)) as Hmemidx.
+  destruct Hmemidx as [Hmemidx [Hmem3 [Hfunc3 [Htab3 Hglob3]]]]; simpl in *.
+
+  assert (Hgvs_len : length gvs = length mod_globals).
+  {
+    rewrite /instantiate_globals in Hinit_globs.
+    simpl in Hinit_globs.
+    apply Forall2_length in Hinit_globs.
+    by symmetry in Hinit_globs.
+  }
+  specialize (alloc_glob_gen_index _ _ _ _ _ Hgvs_len (symmetry Heqs_igs)) as Hglobidx.
+  destruct Hglobidx as [Hglobidx [Hglob4 [Hfunc4 [Htab4 Hmem4]]]]; simpl in *.
+  
+  rewrite <- Hfunc4 in *. rewrite <- Hfunc3 in *. rewrite <- Hfunc2 in *. rewrite -> Hfunc1 in *.
+  rewrite <- Htab4 in *. rewrite <- Htab3 in *. rewrite -> Htab2 in *. rewrite <- Htab1 in *.
+  rewrite <- Hmem4 in *. rewrite -> Hmem3 in *. rewrite <- Hmem2 in *. rewrite <- Hmem1 in *.
+  rewrite -> Hglob4 in *. rewrite <- Hglob3 in *. rewrite <- Hglob2 in *. rewrite <- Hglob1 in *.
+
+  clear Hfunc1 Hfunc2 Hfunc3 Hfunc4.
+  clear Htab1 Htab2 Htab3 Htab4.
+  clear Hmem1 Hmem2 Hmem3 Hmem4.
+  clear Hglob1 Hglob2 Hglob3 Hglob4.
+  clear Heqs_ifs Heqs_its Heqs_ims Heqs_igs.
+
+  remember ((λ mf : module_func, gen_func_instance mf _) <$> mod_funcs) as s_funcs_new.
+  remember (_ <$> map _ mod_tables) as s_tabs_new.
+  remember ((λ '{| lim_min := min; lim_max := maxo |}, _) <$> mod_mems) as s_mems_new.
+  remember (_ <$> combine mod_globals gvs) as s_globs_new.
+
+  split.
   - (* cl_type *)
-    remember ((λ mf : module_func, gen_func_instance mf _) <$> mod_funcs) as s_funcs_new.
     rewrite -> List.Forall_app.
     split.
     + (* forall cl_type_check s' s_funcs0 *)
@@ -446,6 +1328,7 @@ Proof.
       by apply Hcl.
     + (* forall cl_type_check s' s_funcs_new *)
       rewrite List.Forall_forall => fc Hin.
+
       rewrite -> Heqs_funcs_new in Hin.
       rewrite /gen_func_instance in Hin.
       simpl in Hin.
@@ -455,150 +1338,471 @@ Proof.
       rewrite /Coqlib.option_map in Hnth.
       destruct (nth_error mod_funcs n) eqn: Heqm => //=.
       inversion Hnth. clear Hnth.
-      rename H0 into Heq_fc.
-      
+      rename H0 into Heq_fc. 
+
       assert (Hex_ty: exists ty, List.nth_error fts n = Some ty).
       {
         rewrite nth_error_lookup in Heqm.
-        specialize (Forall2_lookup_l _ _ _ _ _  Hftstype Heqm) as H1.
+        specialize (Forall2_lookup_l _ _ _ _ _  HFuncType Heqm) as H1.
         destruct H1 as [ty [Heqy _]].
         rewrite <- nth_error_lookup in Heqy.
         by exists ty.
       }
 
       destruct Hex_ty as [ty Hty].
-      specialize (Forall2_nth_error _ _ _ _ _ n m ty Hftstype Heqm Hty) as Hftstype_n.
+      specialize (Forall2_nth_error _ _ _ _ _ n m ty HFuncType Heqm Hty) as HFuncType_n.
 
       rewrite /typing.cl_type_check_single.
-      destruct ty as [t1s t2s]. 
+      destruct ty as [t1s t2s].
       exists (Tf t1s t2s).
-      remember (Build_t_context mod_types fts nil nil nil nil nil None) as C.
+      remember (Build_t_context mod_types _ _ _ _ nil nil None) as C.
 
       eapply cl_typing_native with (C := C) => //=.
-
-      { (* inst_typing store inst C *)
+      * (* inst_typing *)
         destruct C.
         destruct tc_local => //=.
         destruct tc_label => //=.
         destruct tc_return => //=.
+
         inversion HeqC; subst.
-        destruct HeqC. 
+        clear n m Heqm t1s t2s Hty HFuncType_n.
+
+        specialize (external_typing_aux _ _ _ Himp_typing) as Hvimps_len.
+        destruct Hvimps_len as [Himps_func_len [Himps_glob_len [Himps_tab_len Himps_mem_len]]].
+        
+        apply/andP. split.
+        apply/andP. split.
+        apply/andP. split.
         apply/andP. split => //=.
-        apply/andP. split => //=.
-        apply/andP. split => //=.
-        apply/andP. split => //=.
-        { (* functions_agree *)
-          rewrite /gen_func_instance. simpl.
-          rewrite /typing.functions_agree.
-          eapply all2_and with (g := (fun n0 f => ssrnat.leq (S n0) _)) => //=.
-          split.
-          {
-            rewrite <- Forall2_all2.
-            rewrite List.app_length.
-            rewrite fmap_length.
-            rewrite Hidx.
-            apply Forall_Forall2_l.
-            (*
-              Forall_Forall2_l: ∀ (A B : Type) (P : A → B → Prop) (l : seq.seq A) (k : seq.seq B),
-                length l = length k → Forall (λ x : A, ∀ y : B, P x y) l → Forall2 P l k
-             *)
-            - rewrite gen_index_len.
-              by apply Forall2_length in Hftstype.
-            - rewrite Forall_forall.
-              move => x Hin _.
-              apply gen_index_in in Hin.
-              by move/ssrnat.ltP in Hin.
-          }
-          {
-            clear n m Heqm t1s t2s Hty Hftstype_n.
-            rewrite /module_func_typing in Hftstype; simpl in Hftstype.
-            rewrite <- Forall2_all2.
-            assert (Hlen: length ifs = length mod_funcs).
-            {
-              rewrite <- gen_index_len with (offset := (length s_funcs0)).
-              rewrite <- Hidx.
-              by rewrite map_length.
-            }
-            apply Forall2_lift.
-            - (* length (map (λ '(Mk_funcidx i), i) ifs) = length fts *)
-              rewrite map_length.
-              rewrite Hlen.
-              by apply Forall2_length in Hftstype.
-            - 
-              move => i fidx ft Hfuncs_nth Hfts_nth.
-              assert (Hnth: i < length mod_funcs).
+
+        -- (* functions_agree *) 
+           rewrite /gen_func_instance /typing.functions_agree. simpl.
+           eapply all2_and with (g := (fun n0 f => ssrnat.leq (S n0) _)) => //.
+           assert (Hifs_len: length (map (λ '(Mk_funcidx i), i) ifs) = length mod_funcs).
+           {
+             rewrite <- gen_index_len with (offset := (length s_funcs0)).
+             by rewrite Hfunidx.
+           }
+           specialize (external_typing_aux _ _ _ Himp_typing) as Hvimps_len.
+           split.
+           ++ (* n < length fs *)
+              rewrite <- Forall2_all2. 
+              rewrite List.app_length.
+              rewrite fmap_length.
+              Check Forall_Forall2_l.
+              apply Forall_Forall2_l.
+              ** (* v_imps & t_imps *)
+                 rewrite map_length.
+                 repeat rewrite -> app_length.
+                 rewrite Himps_func_len. f_equal.
+                 replace (length ifs) with (length (map (λ '(Mk_funcidx i), i) ifs)); last by rewrite map_length.
+                 rewrite Hifs_len.
+                 by apply Forall2_length in HFuncType.
+              ** rewrite map_app.
+                 rewrite Forall_app.
+                 split.
+                 *** rewrite Forall_lookup.
+                     move => i n0 Hnth _.
+                     
+                     rewrite ->  Forall2_lookup in Himp_typing.
+                     rewrite map_fmap in Hnth.
+                     rewrite list_lookup_fmap in Hnth.
+                     destruct (ext_funcs v_imps !! i) eqn: Hvimp => //.
+                     simpl in Hnth.
+                     apply ext_funcs_lookup_exist in Hvimp.
+                     destruct Hvimp as [k Hvimp].
+                     specialize (Himp_typing k).
+                     rewrite Hvimp in Himp_typing.
+                     inversion Himp_typing; subst.
+                     destruct f.
+                     inversion Hnth; subst.
+                     inversion H1; subst.
+                     simpl in H2.
+                     apply/ssrnat.ltP. move/ssrnat.ltP in H2.
+                     by lias.
+                 *** rewrite Hfunidx.
+                     rewrite Forall_forall.
+                     move => x Hin _.
+                     apply gen_index_in in Hin.
+                     by move/ssrnat.ltP in Hin.
+           ++ (* cl_type *)
+              rewrite <- Forall2_all2.
+              rewrite map_app.
+              apply Forall2_app.
+              ** apply Forall2_lift; first by rewrite map_length.
+                 move => i v_imp t_imp Hvimps_nth Htimps_nth.
+                 apply/eqP. 
+                 specialize (external_typing_funcs_aux _ _ _ _ _ _ Himp_typing Hvimps_nth Htimps_nth) as Hext_typing. simpl in Hext_typing.
+                 rewrite <- Hext_typing.
+                 f_equal.
+                 apply nth_error_app1.
+                 rewrite /option_map in Hext_typing.
+                 destruct (nth_error s_funcs0 v_imp) eqn: Hfuncs_nth => //.
+                 by eapply nth_error_Some_length.
+              ** rewrite /module_func_typing in HFuncType. simpl in HFuncType.
+                 apply Forall2_lift.
+                 *** (* length (map (λ '(Mk_funcidx i), i) ifs) = length fts *)
+                     rewrite Hifs_len.
+                     by apply Forall2_length in HFuncType.
+                 *** move => i fidx ft Hidxs_nth Hfts_nth.
+                     
+                     specialize (nth_error_same_length_list _ _ _ _ _ _ Hifs_len Hidxs_nth) as Hfuncs_nth.
+                     destruct Hfuncs_nth as [func Hfuncs_nth].
+                     specialize (Forall2_nth_error _ _ _ _ _ _ _ _ HFuncType Hfuncs_nth Hfts_nth) as HFuncType_n.
+                     simpl in HFuncType_n.
+                     destruct func. destruct modfunc_type. destruct ft as [t1s t2s].
+                     destruct HFuncType_n as [_ [Hft _]].
+                     
+                     rewrite Hfunidx in Hidxs_nth.
+                     rewrite nth_error_lookup in Hidxs_nth.
+                     rewrite gen_index_lookup in Hidxs_nth; last by eapply nth_error_Some_length.
+                     inversion Hidxs_nth; subst. clear Hidxs_nth.
+
+                     rewrite nth_error_app2; last by lias.
+                     replace (length s_funcs0 + i - length s_funcs0) with i; last by lias.
+
+                     rewrite nth_error_lookup.
+                     rewrite list_lookup_fmap.
+                     rewrite nth_error_lookup in Hfuncs_nth.
+                     by rewrite Hfuncs_nth.
+        -- (* globals_agree *)
+           rewrite /globals_agree.
+           eapply all2_and with (g := (fun n tg => ssrnat.leq (S n) _)) => //.
+           assert (Higs_len: length (map (λ '(Mk_globalidx i), i) igs) = length mod_globals).
+           {
+             rewrite <- gen_index_len with (offset := length s_globals0).
+             by rewrite Hglobidx.
+           }
+           assert (Hcombine_len: length (combine mod_globals gvs) = length mod_globals).
+           {
+             rewrite combine_length.
+             rewrite Hgvs_len.
+             by rewrite Nat.min_id.
+           }
+           split.
+           ++ (* n < length gs *)
+             rewrite <- Forall2_all2.
+             rewrite List.app_length.
+             rewrite fmap_length.
+             apply Forall_Forall2_l.
+             ** rewrite map_length.
+                repeat rewrite -> app_length.
+                rewrite Himps_glob_len. f_equal.
+                replace (length igs) with (length (map (λ '(Mk_globalidx i), i) igs)); last by rewrite map_length.
+                rewrite Higs_len.
+                by apply Forall2_length in HGlobType.
+             ** rewrite map_app.
+                rewrite Forall_app.
+                split.
+                *** rewrite Forall_lookup.
+                    move => i n0 Hnth _.
+                    
+                    rewrite map_fmap in Hnth.
+                    rewrite list_lookup_fmap in Hnth.
+                    destruct (ext_globs v_imps !! i) eqn: Hvimp => //.
+                    simpl in Hnth.
+                    apply ext_globs_lookup_exist in Hvimp.
+                    destruct Hvimp as [k Hvimp].
+
+                    rewrite -> Forall2_lookup in Himp_typing.
+                    specialize (Himp_typing k).
+                    rewrite Hvimp in Himp_typing.
+                    inversion Himp_typing; subst.
+                    
+                    destruct g.
+                    inversion Hnth; subst.
+                    inversion H1; subst.
+                    simpl in H2.
+                    apply/ssrnat.ltP. move/ssrnat.ltP in H2.
+                    by lias.
+                *** rewrite Hglobidx.
+                    rewrite Forall_forall.
+                    move => x Hin _.
+                    apply gen_index_in in Hin.
+                    rewrite Hcombine_len.
+                    by move/ssrnat.ltP in Hin.
+           ++ (* global_agree *) 
+              rewrite <- Forall2_all2.
+              rewrite map_app.
+              apply Forall2_app.
+              ** apply Forall2_lift; first by rewrite map_length.
+                 move => i v_imp t_imp Hvimps_nth Htimps_nth.
+                 apply/eqP.
+                 specialize (external_typing_globs_aux _ _ _ _ _ _ Himp_typing Hvimps_nth Htimps_nth) as Hext_typing. simpl in Hext_typing.
+                 rewrite <- Hext_typing.
+                 f_equal.
+                 apply nth_error_app1.
+                 rewrite /option_map in Hext_typing.
+                 destruct (nth_error s_globals0 v_imp) eqn: Hglobs_nth => //.
+                 by eapply nth_error_Some_length.
+              ** rewrite /module_glob_typing in HGlobType. simpl in HGlobType.
+                 apply Forall2_lift.
+                 *** (* length (map (λ '(Mk_globalidx i), i) igs) = length gts *)
+                     rewrite Higs_len.
+                     by apply Forall2_length in HGlobType.
+                 *** move => i gidx gt Hidxs_nth Hgts_nth.
+
+                     specialize (nth_error_same_length_list _ _ _ _ _ _ Higs_len Hidxs_nth) as Hglobs_nth.
+                     destruct Hglobs_nth as [glob Hglobs_nth].
+                     specialize (Forall2_nth_error _ _ _ _ _ _ _ _ HGlobType Hglobs_nth Hgts_nth) as HGlobType_n.
+                     simpl in HGlobType_n.
+                     destruct glob.
+                     destruct HGlobType_n as [_ [Hgt _]]. subst.
+
+                     rewrite Hglobidx in Hidxs_nth.
+                     rewrite nth_error_lookup in Hidxs_nth.
+                     rewrite gen_index_lookup in Hidxs_nth; last by eapply nth_error_Some_length.
+                     inversion Hidxs_nth; subst. clear Hidxs_nth.
+
+                     rewrite nth_error_app2; last by lias.
+                     replace (length s_globals0 + i - length s_globals0) with i; last by lias.
+                     
+                     rewrite nth_error_lookup.
+                     rewrite list_lookup_fmap.
+
+                     specialize (nth_error_same_length_list _ _ _ _ _ _ (symmetry Hgvs_len) Hglobs_nth) as Hgvs_nth.
+                     destruct Hgvs_nth as [gv Hgvs_nth].
+                     assert (Hcombine : (combine mod_globals gvs) !! i = Some ({| modglob_type := modglob_type; modglob_init := modglob_init |}, gv)).
+                     {
+                       rewrite <- nth_error_lookup.
+                       rewrite -> nth_error_nth' with (d := ({| modglob_type := modglob_type; modglob_init := modglob_init |}, gv)); last by rewrite Hcombine_len; eapply nth_error_Some_length.
+                       rewrite combine_nth => //.
+                       by repeat erewrite nth_error_nth => //. 
+                     }
+                     rewrite Hcombine. simpl.
+                     rewrite /global_agree. simpl.
+                     apply/eqP. f_equal.
+                     apply/andP. split => //.
+                     apply/eqP.
+                     
+                     rewrite /instantiate_globals in Hinit_globs. simpl in Hinit_globs.
+                     rewrite -> Forall2_lookup in Hinit_globs.
+                     specialize (Hinit_globs i).
+                     rewrite nth_error_lookup in Hglobs_nth.
+                     rewrite nth_error_lookup in Hgvs_nth.
+                     rewrite Hglobs_nth in Hinit_globs.
+                     rewrite Hgvs_nth in Hinit_globs.
+                     inversion Hinit_globs; subst. clear Hinit_globs.
+                     simpl in H1.
+                     
+                     rewrite -> Forall2_lookup in HGlobType.
+                     specialize (HGlobType i).
+                     rewrite nth_error_lookup in Hgts_nth.
+                     rewrite Hgts_nth in HGlobType.
+                     rewrite Hglobs_nth in HGlobType.
+                     inversion HGlobType; subst. clear HGlobType.
+
+                     destruct H2 as [Hconst_exprs [_ Hbe_typing]].
+                     specialize (const_exprs_impl _ _ _ Hconst_exprs Hbe_typing) as Hexprs.
+                     clear Hconst_exprs.
+                     destruct Hexprs as [expr [Hexpr Hconst]].
+                     rewrite /const_expr in Hconst. simpl in Hconst.
+                     rewrite -> Hexpr in *.  clear Hexpr.
+                     destruct expr; simpl in * => //.
+                     { (* modglob_init = [BI_get_global i0] *)
+
+                       Search BI_get_global.
+
+                       (* [BI_get_global i0] ->* gv *)
+                       Search s_globals.
+                       apply reduce_trans_get_global in H1.
+                       rewrite /sglob_val /sglob /sglob_ind in H1.
+                       simpl in H1.
+                       rewrite /option_map in H1.
+                       destruct (option_bind _ _) eqn: Heq1 => //.
+                       inversion H1.
+                       rewrite <- H0 in *. clear H1 H0.
+                       rewrite /option_bind in Heq1.
+                       destruct (nth_error (map _ _) i0) eqn: Heq2 => //.
+
+                       (* [BI_get_global i0] has type modglob_type *)
+                       eapply Get_global_typing in Hbe_typing => //.
+                       simpl in Hbe_typing.
+                       destruct Hbe_typing as [ty [H1 [H2 _]]].
+                       inversion H2; subst.
+                       rewrite /option_map in H1.
+                       destruct (nth_error (ext_t_globs t_imps) i0) eqn: Htl => //.
+
+                       (* todo: create a lemma nth_error (map f l) i = f <$> l !! i*)
+                       rewrite nth_error_lookup in Heq2.
+                       rewrite map_fmap in Heq2.
+                       rewrite list_lookup_fmap in Heq2.
+                       assert (Heq3: (ext_globs v_imps ++ igs) !! i0 = ext_globs v_imps !! i0).
+                       { apply nth_error_Some_length in Htl.
+                         rewrite <- Himps_glob_len in Htl.
+                         eapply nth_error_app1 with (l' := igs) in Htl.
+                         by repeat rewrite nth_error_lookup in Htl.
+                       }
+                       replace ((ext_globs v_imps ++ igs) !! i0) with (ext_globs v_imps !! i0) in Heq2.
+                       rewrite <- list_lookup_fmap in Heq2.
+                       rewrite <- map_fmap in Heq2.
+                       rewrite <- nth_error_lookup in Heq2.
+                       specialize (external_typing_globs_aux _ _ _ _ _ _ Himp_typing Heq2 Htl) as Htyping. simpl in Htyping.
+                       rewrite /option_map in Htyping.
+                       destruct (nth_error s_globals0 g0) eqn: Heq4 => //.
+                       inversion Htyping. clear Htyping.
+                       rewrite /global_agree in H0.
+                       Check nth_error_Some_length.
+                       specialize (nth_error_Some_length _ _ _ _ Heq4) as Hg0.
+                       eapply nth_error_app1 in Hg0. rewrite Hg0 in Heq1.
+                       rewrite Heq4 in Heq1. inversion Heq1; subst.
+                       inversion H1; subst.
+                       move/andP in H0. destruct H0 as [_ H0].
+                       by move/eqP in H0.                     
+                     }
+                     { (* modglob_init = [BI_const v] *)
+                       apply reduce_trans_const in H1. subst.
+                       Search BI_const.
+                       apply BI_const_typing in Hbe_typing.
+                       simpl in Hbe_typing. by inversion Hbe_typing.
+                     }
+        -- (* tabi_agree *) 
+           rewrite <- Forall2_all2.
+           rewrite map_app.
+           apply Forall2_app.
+           ** apply Forall2_lift; first by rewrite map_length.
+              move => i v_imp t_imp Hvimps_nth Htimps_nth.
+              specialize (external_typing_tabs_aux _ _ _ _ _ _ Himp_typing Hvimps_nth Htimps_nth) as Hext_typing. simpl in Hext_typing.
+              by eapply tabi_agree_aux.
+           ** assert (Hits_len: length (map (λ '(Mk_tableidx i), i) its) = length mod_tables).
               {
-                rewrite Coqlib.list_map_nth in Hfuncs_nth.
-                destruct (List.nth_error ifs i) eqn:Hnth_i => //=.
-                assert (H: List.nth_error ifs i <> None) by rewrite Hnth_i => //.
-                apply List.nth_error_Some in H.
-                by rewrite <- Hlen.
+                rewrite <- gen_index_len with (offset := length s_tables0).
+                rewrite Htabidx.
+                by rewrite map_length.
               }
-              rewrite Hidx in Hfuncs_nth.
-              rewrite nth_error_lookup in Hfuncs_nth.
-              rewrite gen_index_lookup in Hfuncs_nth => //.
-              (* todo: length l1 = length l2 -> l1 !! i = Some m -> exists, l2 !! i = Some n *)
-              apply List.nth_error_Some in Hnth.
-              destruct (List.nth_error mod_funcs i) eqn: Hmod_funcs_i => //=.
-              clear Hnth.
-              specialize (Forall2_nth_error _ _ _ _ _ _ _ _ Hftstype Hmod_funcs_i Hfts_nth) as Hftstype_n.
-              simpl in Hftstype_n.
-              simpl in Hfuncs_nth.
-              destruct m. destruct modfunc_type. destruct ft as [t1s t2s].
-              destruct Hftstype_n as [_ [Hft _]].
-              inversion Hfuncs_nth; subst.
-              clear Hfuncs_nth.
-              rewrite nth_error_app2; last by lias.
-              Search "-".
-              replace (length s_funcs0 + i - length s_funcs0) with i; last by lias.
-              Search fmap lookup.
-              rewrite nth_error_lookup.
-              rewrite list_lookup_fmap.
-              rewrite nth_error_lookup in Hmod_funcs_i.
-              rewrite Hmod_funcs_i. by simpl.
-          }
-        }
-    }
-    { (* the type index of function m references type (Tf t1s t2s) in mod_types *)
-      rewrite /module_func_typing in Hftstype_n.
-      destruct m. simpl.
-      destruct modfunc_type as [i].
-      destruct Hftstype_n as [_ [Hnth _]].
-      move/eqP in Hnth.
-      rewrite <- Hnth.
-      by inversion HeqC.
-    }
-    { (* be_typing *)
-      rewrite /module_func_typing in Hftstype_n.
-      rewrite /upd_local_label_return.
-      destruct m. simpl.
-      destruct modfunc_type.
-      destruct Hftstype_n as [_ [_ Hbe_typing]].
-      by apply Hbe_typing.
-    }
+              apply Forall2_lift.
+              *** rewrite Hits_len.
+                  by rewrite map_length.
+              *** move => i tidx tt Hidxs_nth Htts_nth.
+
+                  rewrite Htabidx in Hidxs_nth.
+                  rewrite nth_error_lookup in Hidxs_nth.
+                  rewrite gen_index_lookup in Hidxs_nth; last by eapply nth_error_Some_length.
+                  inversion Hidxs_nth; subst. clear Hidxs_nth.
+                  
+                  rewrite /tabi_agree.
+                  apply/andP. split.
+
+                  {
+                    apply /ssrnat.ltP.
+                    rewrite app_length.
+                    apply plus_lt_compat_l.
+                    rewrite fmap_length.
+                    by eapply nth_error_Some_length.
+                  }
+                  {
+                    rewrite nth_error_app2; last by lias.
+                    replace (length s_tables0 + i - length s_tables0) with i; last by lias.
+
+                    rewrite nth_error_lookup.
+                    rewrite list_lookup_fmap.
+                    rewrite <- nth_error_lookup.
+                    rewrite Htts_nth.
+                    
+                    destruct tt. destruct tt_limits. simpl.
+                    rewrite /tab_typing. simpl.
+                    apply/andP. split => //=.
+                    rewrite /tab_size. simpl. 
+                    by rewrite repeat_length.
+                  }
+        -- (* memi_agree *)
+           rewrite <- Forall2_all2.
+           rewrite map_app.
+           assert (Hims_len: length (map (λ '(Mk_memidx i), i) ims) = length mod_mems).
+           {
+             rewrite <- gen_index_len with (offset := length s_mems0).
+             by rewrite Hmemidx.
+           }
+           apply Forall2_app.
+           ** apply Forall2_lift; first by rewrite map_length.
+              move => i v_imp t_imp Hvimps_nth Htimps_nth.
+              specialize (external_typing_mems_aux _ _ _ _ _ _ Himp_typing Hvimps_nth Htimps_nth) as Hext_typing. simpl in Hext_typing.
+              by eapply memi_agree_aux.            
+           ** rewrite /module_mem_typing in HMemType.
+              apply Forall2_lift; first by rewrite Hims_len.
+              move => i midx mt Hidxs_nth Hmts_nth.
+
+              rewrite Hmemidx in Hidxs_nth.
+              rewrite nth_error_lookup in Hidxs_nth.
+              rewrite gen_index_lookup in Hidxs_nth; last by eapply nth_error_Some_length.
+              inversion Hidxs_nth; subst. clear Hidxs_nth.
+
+              rewrite /memi_agree.
+              apply/andP. split.
+
+              {
+                apply /ssrnat.ltP.
+                rewrite app_length.
+                apply plus_lt_compat_l.
+                rewrite fmap_length.
+                by eapply nth_error_Some_length.
+              }
+              {
+                rewrite nth_error_app2; last by lias.
+                replace (length s_mems0 + i - length s_mems0) with i; last by lias.
+
+                rewrite nth_error_lookup.
+                rewrite list_lookup_fmap.
+                rewrite <- nth_error_lookup.
+                (* todo: nth_error (f <$> l) i = f <$> nth_error l i *)
+                rewrite Hmts_nth.
+
+                destruct mt. 
+                rewrite /mem_typing. simpl.
+                apply/andP. split => //=.
+                rewrite /mem_size /operations.mem_length /memory_list.mem_length. simpl.
+                destruct lim_min => //.
+                rewrite /page_size. simpl.
+                rewrite repeat_length.
+                rewrite positive_nat_N. 
+
+                assert (Hdiv: N.div (N.pos (64 * 1024 * p)) (N.pos (64 * 1024)) = N.pos p).
+                {
+                  replace (N.pos (64 * 1024 * p)) with (N.mul (N.pos (64 * 1024)) (N.pos p)); last by simpl.
+                  rewrite N.mul_comm.
+                  by apply N.div_mul => //.
+                }
+                rewrite Hdiv.
+                by rewrite N.leb_refl.
+              }
+      * (* the type index of function m references type (Tf t1s t2s) in mod_types *)
+        rewrite /module_func_typing in HFuncType_n.
+        destruct m. simpl.
+        destruct modfunc_type as [i].
+        destruct HFuncType_n as [_ [Hnth _]].
+        move/eqP in Hnth.
+        rewrite <- Hnth.
+        by inversion HeqC.
+      * (* be_typing *)
+        rewrite /module_func_typing in HFuncType_n.
+        rewrite /upd_local_label_return.
+        destruct m. simpl.
+        destruct modfunc_type.
+        destruct HFuncType_n as [_ [_ Hbe_typing]].
+        by apply Hbe_typing. 
   split.
   - (* tab_agree *)
-    apply List.Forall_forall => tab Hin.
-    rewrite -> List.Forall_forall in Htab_agree.
-    apply tab_agree_aux.
-    by apply Htab_agree.
+    rewrite Forall_app.
+    split.
+    + (* forall tab_agree s' s_tables0 *)
+      apply Forall_forall => ti Hin.
+      rewrite -> Forall_forall in Htab_agree.
+      apply tab_agree_aux.
+      by apply Htab_agree.
+    + (* forall tab_agree s' s_tabs_new *)
+      by eapply tab_agree_from_typing.
   - (* mem_agree *)
-    assumption. 
+    rewrite Forall_app.
+    split.
+    + (* forall mem_agree s_mems0 *)
+      by exact Hmem_agree.
+    + (* forall mem_agree s_mems_new *)
+      by eapply mem_agree_from_typing.
 Admitted.
 
-Definition module_restriction (m: module) : Prop :=
-  m.(mod_tables) = [::] /\
-  m.(mod_mems) = [::] /\
-  m.(mod_globals) = [::] /\
-  m.(mod_elem) = [::] /\
-  m.(mod_data) = [::] /\
-  m.(mod_start) = None /\
-  m.(mod_imports) = [::] /\
-  m.(mod_exports) = [::].
-
+  
 Lemma instantiation_sound_simpl:  forall (s: store_record) m v_imps s' inst v_exps start,
   store_typing s ->
-  module_restriction m ->
   instantiate s m v_imps ((s', inst, v_exps), start) ->
   (store_typing s').
   (* (exists C, inst_typing s' inst C) /\
@@ -606,91 +1810,29 @@ Lemma instantiation_sound_simpl:  forall (s: store_record) m v_imps s' inst v_ex
   (pred_option (fun i => i < length s'.(s_funcs)) start).*)
   (* /\ store_extension s s' *)
 Proof.
-  move => s m v_imps s' inst v_exps start HStoreType HRestr HInst.
-
-  (* Extract the artificial constraints we're imposing on the module *)
-  unfold module_restriction in HRestr.
-  destruct m => /=.
-  simpl in HRestr.
-  destruct HRestr as [-> [-> [-> [-> [-> [-> [-> ->]]]]]]].
+  move => s m v_imps s' inst v_exps start HStoreType HInst.
 
   unfold instantiate, instantiation.instantiate in HInst.
-  destruct HInst as [t_imps [t_exps [hs' [s'_end [? [? [? [HModType [HImpType [HAllocModule H]]]]]]]]]].
+  destruct HInst as [t_imps [t_exps [hs' [s'_end [g_inits [e_offs [d_offs [HModType [HImpType [HAllocModule H]]]]]]]]]].
 
   destruct H as [HInstGlob [HInstElem [HInstData [HBoundElem [HBoundData [HStart HStore]]]]]].
   simpl in *.
 
-  (* There are a lot of hypotheses here, but almost all of them simplify to a trivial condition due to the current constraint on the module. *)
-
-  (* HInstGlob *)
-  unfold instantiate_globals in HInstGlob.
-  simpl in HInstGlob.
-  inversion HInstGlob; subst; clear HInstGlob.
-
-  (* HInstElem *)
-  unfold instantiate_elem in HInstElem.
-  simpl in HInstElem.
-  inversion HInstElem; subst; clear HInstElem.
-
-  (* HInstData *)
-  unfold instantiate_data in HInstData.
-  simpl in HInstData.
-  inversion HInstData; subst; clear HInstData.
-
-  (* HBoundData *)
-  unfold check_bounds_data in HBoundData.
-  simpl in HBoundData.
-  (* this is vacuously true. *)
-  clear HBoundData.
-
-  (* HBoundElem *)
-  unfold check_bounds_elem in HBoundElem.
-  simpl in HBoundElem.
-  clear HBoundElem.
-
-  (* HCheckStart *)
-  unfold check_start in HStart.
-  simpl in HStart.
-  move/eqP in HStart; subst.
-
-  (* HStore *)
-  unfold init_mems, init_tabs in HStore.
-  simpl in HStore.
-  move/eqP in HStore; subst.
-
-  (* HModType *)
-  (* This is an important part -- it gives a lot of validity information of the function references. *)
-  unfold module_typing in HModType.
-  destruct HModType as [fts [gts [HFuncType [_ [_ [HGlobType [_ [_ [_ [HImpValid _]]]]]]]]]].
-  simpl in *.
-  inversion HGlobType; subst; clear HGlobType.
-  inversion HImpValid; subst; clear HImpValid.
-  repeat rewrite List.app_nil_r in HFuncType.
-
-  (* We know v_imps is empty as well *)
-  inversion HImpType; subst; clear HImpType.
-  simpl in *.
+  specialize (alloc_module_sound _ _ _ _ _ _ _ _ _ _ HAllocModule HModType HImpType HInstGlob HStoreType) as Htyping. rename s'_end into s1.
   
-
-  (* Now, extract information from alloc_module. *)
-  remember (alloc_funcs host_function s mod_funcs inst) as s_ifs.
-  destruct s_ifs as [s' ifs].
-  destruct inst.
-  repeat (move/andP in HAllocModule; destruct HAllocModule as [HAllocModule ?]).
-  simpl in *.
-  move/eqP in H; subst.
-  move/eqP in H0; subst.
-  move/eqP in H1; subst.
-  move/eqP in H2; subst.
-  move/eqP in H3; subst.
-  move/eqP in H4; subst.
-  move/eqP in HAllocModule; subst.
-  repeat rewrite List.app_nil_r in Heqs_ifs.
-
-  (* We've reached the original simplified version we want, but with a much better shape of the lemma now for future extension. *)
-
-  by eapply alloc_func_sound; eauto => //.
+  remember (init_tabs host_function s1 inst [seq Z.to_nat (Wasm_int.Int32.intval o) | o <- e_offs] (mod_elem m)) as s2. 
+  specialize (init_tabs_preserve _ _ _ _ _ (symmetry Heqs2)) as Hs2.
+  destruct Hs2 as [_[Hs2_mems _]].
   
- 
-Admitted.
+  eapply init_tabs_preserve_typing with (s' := s2) in Htyping => //.
+  rewrite Heqs2 in Htyping. 
+  
+  move/eqP in HStore.
+
+  rewrite /check_bounds_data in HBoundData.
+  rewrite Hs2_mems in HBoundData.
+  rewrite HStore.
+  eapply init_mems_preserve_typing => //.
+  by rewrite Heqs2.
+Qed.
 
